Working on applying unique_child in property 2 proof

SymbolicExecution.v
@@ -52,55 +52,55 @@ Inductive node_eval (prog: Program) : TreeNode -> list TreeNode -> Prop :=
   
   | E_Assign : forall x ie st pc n path,
     let se := (makeSymbolicInt st ie) in
-    let node := <<st, pc, n>> in
-    let node' := <<(x, se) :: st, pc, (nextInstruction (stmts prog) n)>> in
+    let parent := <<st, pc, n>> in
+    let child := <<(x, se) :: st, pc, (nextInstruction (stmts prog) n)>> in
     (findStatement (stmts prog) n) = <{x := ie}> ->
-    node_eval prog node path ->
-    node_eval prog node' (node' :: path)
+    node_eval prog parent path ->
+    node_eval prog child (child :: path)
 
    | E_IfThen : forall be then_body else_body st pc n path,
     let sbe := (makeSymbolicBool st be) in
-    let node := <<st, pc, n>> in
-    let node' := <<st, sbe::pc, (n+1)>> in
+    let parent := <<st, pc, n>> in
+    let child := <<st, sbe::pc, (n+1)>> in
     (findStatement (stmts prog) n) = <{if be then then_body else else_body end}> ->
     (makeSymbolicBool st be) = sbe ->
     (SAT (sbe::pc)) ->
-    node_eval prog node path ->
-    node_eval prog node' (node' :: path)
+    node_eval prog parent path ->
+    node_eval prog child (child :: path)
 
   | E_IfElse : forall be then_body else_body st pc n path,
     let sbe := (makeSymbolicBool st be) in
-    let node := <<st, pc, n>> in
-    let node' := << st, (<[~sbe]>)::pc, (n + (progLength then_body))>> in
+    let parent := <<st, pc, n>> in
+    let child := << st, (<[~sbe]>)::pc, (n + (progLength then_body))>> in
     (findStatement (stmts prog) n) = <{if be then then_body else else_body end}> ->
     (SAT (<[~sbe]>::pc)) ->
-    node_eval prog node path ->
-    node_eval prog node' (node' :: path)
+    node_eval prog parent path ->
+    node_eval prog child (child :: path)
 
    | E_GoTo: forall pos st pc n path,
-    let node := << st, pc, n>> in
-    let node' := <<st, pc, pos>> in
+    let parent := << st, pc, n>> in
+    let child := <<st, pc, pos>> in
     (findStatement (stmts prog) n) = <{go_to pos}> ->
-    node_eval prog node path ->
-    node_eval prog node' (node' :: path)
+    node_eval prog parent path ->
+    node_eval prog child (child :: path)
 
   | E_WhileBody: forall be body st pc n path,
     let sbe := (makeSymbolicBool st be) in
-    let node := <<st, pc, n>> in
-    let node' := <<st, sbe::pc, (n + 1)>> in
+    let parent := <<st, pc, n>> in
+    let child := <<st, sbe::pc, (n + 1)>> in
     (findStatement (stmts prog) n) = <{while be do body end}> ->
     (SAT (sbe:: pc)) ->
-    node_eval prog node path ->
-    node_eval prog node' (node' :: path)
+    node_eval prog parent path ->
+    node_eval prog child (child :: path)
 
  | E_WhileSkip: forall be body st pc n path,
     let sbe := (makeSymbolicBool st be) in
-    let node := <<st, pc, n>> in
-    let node' := << st, (<[~sbe]>:: pc), (n + (progLength body) + 1)>> in
+    let parent := <<st, pc, n>> in
+    let child := << st, (<[~sbe]>:: pc), (n + (progLength body) + 1)>> in
     (findStatement (stmts prog) n) = <{while be do body end}> ->
     (SAT (<[~sbe]>:: pc)) ->
-    node_eval prog node path ->
-    node_eval prog node' (node' :: path).
+    node_eval prog parent path ->
+    node_eval prog child (child :: path).
 
 (** This is stating
     that if a superset of a condition is satisfiable, then the condition itself is 
@@ -255,15 +255,15 @@ Qed.
 (* Definition ancestor (prog: Program) (node1 node2: TreeNode) (path2: list TreeNode): Prop :=
   node_eval prog node2 path2 /\ In node1 path2. *)
 
-Definition ancestor (prog: Program) (node1 node2: TreeNode) : Prop :=
-  exists path2, node_eval prog node2 path2 /\ In node1 path2.
+Definition ancestor (prog: Program) (node1 node2: TreeNode) (path2: list TreeNode): Prop :=
+  node_eval prog node2 path2 /\ In node1 path2.
 
-Lemma ancestor_eval : forall prog node1 node2,
-  ancestor prog node1 node2 -> exists path1, node_eval prog node1 path1.
+Lemma ancestor_eval : forall prog node1 node2 path2,
+  ancestor prog node1 node2 path2 -> exists path1, node_eval prog node1 path1.
 Proof.
-  intros. destruct H as [path2 [H H0]]. remember H as E. clear HeqE.
+  intros. destruct H as [H H0]. remember H as E. clear HeqE.
   induction H; destruct H0;
-  try (exists (node' :: path); rewrite <- H0; easy);
+  try (exists (child :: path); rewrite <- H0; easy);
   try (apply IHnode_eval; easy).
   - exists [<<st, [], 0>>]. rewrite <- H. apply E_Empty.
   - destruct H.
@@ -273,11 +273,11 @@ Qed.
     try (apply IHnode_eval in H0; apply H0).
 Qed. *)
 
-Lemma pathcond_extend : forall prog node1 node2,
-  (ancestor prog node1 node2) ->
+Lemma pathcond_extend : forall prog node1 node2 path2,
+  (ancestor prog node1 node2 path2) ->
   exists path_subset, extractPathCond node2 = path_subset ++ extractPathCond node1.
 Proof. Admitted.
-  (* intros. destruct H. induction H; destruct H0; try (rewrite <- H0);
+(* intros. destruct H. induction H; destruct H0; try (rewrite <- H0);
     try (exists nil; simpl; unfold node; reflexivity);
     try (apply IHnode_eval in H0; apply H0).
   - exists [sbe]; reflexivity.
@@ -313,41 +313,26 @@ Proof.
     rewrite <- H3 in H4. apply H4.
 Qed.
 
-Theorem property_2_simpler : forall prog node1 node2,
-  ancestor prog node1 node2 ->
-  SAT ((extractPathCond node1) ++ (extractPathCond node2)).
-Proof.
-  intros. remember H as H1. clear HeqH1.
-  apply pathcond_extend in H1. destruct H1 as [p H0].
-  rewrite H0. apply SAT_comm.
-  unfold ancestor in H. destruct H as [path2 [H _]].
-  apply property_1 in H. rewrite H0 in H.
-  apply SAT_terms in H. destruct H as [cs H].
-  apply SAT_terms. exists cs; intros. apply in_app_or in H1.
-  destruct H1. apply H in H1. easy.
-  apply H. apply in_or_app. right. easy.
-Qed.
-
 Lemma not_ancestor_not_path : forall prog node1 path1 node2 path2,
   node_eval prog node1 path1 ->
   node_eval prog node2 path2 ->
-  ~(ancestor prog node1 node2) ->
-  ~(ancestor prog node2 node1) ->
+  ~(ancestor prog node1 node2 path2) ->
+  ~(ancestor prog node2 node1 path1) ->
   ~(In node1 path2) /\ ~(In node2 path1).
 Proof.
   intros. unfold ancestor in *. split.
-  - intro. apply H1. exists path2. split.
+  - intro. apply H1. split.
     apply H0. apply H3.
-  - intro. apply H2. exists path1. split.
+  - intro. apply H2. split.
     apply H. apply H3.
 Qed.
 
-Lemma pc_ancestor : forall prog node1 node2 sbe,
-  ancestor prog node1 node2 ->
+Lemma pc_ancestor : forall prog node1 node2 path2 sbe,
+  ancestor prog node1 node2 path2 ->
   In sbe (extractPathCond node1) ->
   In sbe (extractPathCond node2).
 Proof.
-  intros. destruct H as [path2 [H H1]]. induction H; destruct H1;
+  intros. destruct H as [H H1]. induction H; destruct H1;
   try (rewrite <- H in H0; simpl in H0; apply H0; apply H);
   try (subst; apply H0);
   try (simpl; right);
@@ -377,40 +362,40 @@ Proof.
     + intros child Hchild.
       inversion Hchild.
       * apply base_path in H0. rewrite <- H3 in H0. destruct H0.
-      * simpl in *. assert (node = <<s, pc, index>>).
+      * simpl in *. assert (parent = <<s, pc, index>>).
         { apply (unique_path_head prog _ _ path); easy. }
-        simpl in *. subst. unfold node in H5. injection H5. intros.
+        simpl in *. subst. unfold parent in H5. injection H5. intros.
         subst. unfold stmt in H. rewrite H in H2. inversion H2.
 Admitted.
 
 Theorem property_2 : forall prog node1 node2 path1 path2, 
 (node_eval prog node1 path1) -> 
 (node_eval prog node2 path2) ->
-  ~(ancestor prog node1 node2) ->
-  ~(ancestor prog node2 node1) ->
+  ~(ancestor prog node1 node2 path2) ->
+  ~(ancestor prog node2 node1 path1) ->
   ~ (SAT (( extractPathCond node1) ++ (extractPathCond node2))).
 Proof.
-  intros. intros H4.
+
+  intros. intros H4. unfold ancestor in H1. apply not_and_or in H1.
   (** Since we have assumed that both nodes are in the relation, we need to
       unfold the ancestor definition to get that neither node is in the other's path. *)
-  assert (~(In node1 path2) /\ ~(In node2 path1)).
-  { apply (not_ancestor_not_path prog node1 path1 node2 path2); auto. }
-  destruct H3.
-  (* apply SAT_terms in H4. destruct H4 as [cs H4]. *)
+  destruct H1. apply H1. apply H0.
+  unfold ancestor in H2. apply not_and_or in H2.
+  destruct H2. apply H2. apply H. remember H as E. clear HeqE.
   (** Now we can proceed by induction on H. *)
   induction H; intros.
-    - apply base_path in H0. apply H3 in H0. apply H0.
+
+  (* apply SAT_terms in H4. destruct H4 as [cs H4]. *)
+    - apply base_path in H0. apply H1 in H0. apply H0.
     - apply IHnode_eval; auto.
-      + clear IHnode_eval. clear H4. intro Hc. destruct Hc.
-        induction pc.
-        * simpl in *.
-        assert (node = node2). { apply (path_head prog node node' node2 path path2); easy. } rewrite <- H in H2. destruct H2.
-        right. apply (node_path prog). apply H3.
-        + intro Hc. destruct H2. right. apply Hc.
-    -
-    (* - apply IHnode_eval. admit. intros HI. apply H2. right. apply HI.
-      simpl in *. apply H3.
-    -  *)
+      clear IHnode_eval. clear H4.
+      + intro. assert (exists! child', node_eval prog child' (child' :: path)).
+      { apply (unique_child _ parent _). right. exists x, ie; easy. easy. }
+      destruct H5 as [child' [H5 H6]].
+      apply (H6 child) in E. subst.
+      assert (parent = node2).
+      (** We know path2 = node2 :: tail, so then destruct H4 and show that parent has to be at the head or there's a contradiction with H1. *)
+      {  }
 
 
 (* ==================== End: Proof of Property 2 ===================== *)
